{-# OPTIONS --safe --without-K #-}

open import Semantics.Category.Base
open import Semantics.Category.Cartesian
open import Semantics.Category.CartesianClosed
open import Semantics.Category.StrongFunctor

open import Data.Product using (∃; _,_; -,_) renaming (_×_ to _∧_; proj₁ to fst; proj₂ to snd)

open import Relation.Binary.PropositionalEquality using (_≡_; refl; subst)

module Semantics.Category.Evaluation.Functor.Properties
  (C     : Category)
  (isCC  : IsCartesian C)
  (isCCC : IsCartesianClosed C isCC)
  (hasSF : HasStrongFunctor C isCC)
  (ι'    : Category.Obj C)
  where

open Category C
open IsCartesian isCC
open IsCartesianClosed isCCC
open HasStrongFunctor hasSF

Ty'  = Obj
Ctx' = Obj

open import Level using (0ℓ)

open import Relation.Binary using (IsEquivalence; Setoid)

import Relation.Binary.Reasoning.Setoid as EqReasoning

open import Functor.Term
open import Functor.Term.Reduction

open import Semantics.Category.Evaluation.Functor.Base
   C isCC isCCC hasSF
  renaming (module Eval to FunctorBaseEval)

open FunctorBaseEval ι'

abstract
  evalWk-pres-id : ∀ (Γ : Ctx) → evalWk idWk[ Γ ] ≈̇ id'
  evalWk-pres-id []          = ≈̇-sym []'-eta
  evalWk-pres-id Γ@(Γ' `, a) = let open EqReasoning (Sub'-setoid Γ Γ) in begin
    evalWk (keep[ a ] idWk[ Γ' ])             ≈⟨ ×'-map-pres-≈̇-left (evalWk-pres-id Γ') id'[ evalTy a ] ⟩
    id'[ evalCtx Γ' ] ×'-map id'[ evalTy a ]  ≈⟨ ×'-map-pres-id' ⟩
    id'[ evalCtx Γ ]                          ∎

  evalWk-pres-∘-π₁ : evalWk (drop[ a ] w) ≈̇ evalWk w ∘ π₁'[ evalTy a ]
  evalWk-pres-∘-π₁ = ≈̇-refl

  evalWk-pres-×-map-id : evalWk (keep[ a ] w) ≈̇ evalWk w ×'-map id'[ evalTy a ]
  evalWk-pres-×-map-id = ≈̇-refl

  evalWk-pres-π₁ : ∀ (Γ : Ctx) (a : Ty) → evalWk (freshWk {Γ} {a}) ≈̇ π₁'[ evalTy a ]
  evalWk-pres-π₁ Γ a = let open EqReasoning (Sub'-setoid (Γ `, a) Γ) in begin
    evalWk (freshWk {Γ} {a})              ≈⟨ ∘-pres-≈̇-left (evalWk-pres-id Γ) π₁'[ evalTy a ] ⟩
    id'[ evalCtx Γ ] ∘ π₁'[ evalTy a ]  ≈⟨ id'-unit-left (evalCtx Γ) π₁'[ evalTy a ] ⟩
    π₁'[ evalTy a ]                     ∎

module _ {a : Ty} where
  abstract
    evalVar-pres-∘ : ∀ (w : Γ ⊆ Δ) (n : Var Γ a) → evalVar (wkVar w n) ≈̇ evalVar n ∘ evalWk w
    evalVar-pres-∘ (drop {Δ = Δ} {b} w) v = let open EqReasoning (Tm'-setoid (Δ `, b) a) in begin
      evalVar (wkVar (drop[ b ] w) v)                     ≈⟨ ∘-pres-≈̇-left (evalVar-pres-∘ w v) π₁'[ evalTy b ] ⟩
      (evalVar v ∘ evalWk w) ∘ π₁'[ evalTy b ]            ≈⟨ ∘-assoc (evalVar v) (evalWk w) π₁'[ evalTy b ] ⟩
      evalVar v ∘ evalWk (drop[ b ] w)                    ∎
    evalVar-pres-∘ (keep {Δ = Δ} {a} w) (zero {Γ}) = let open EqReasoning (Tm'-setoid (Δ `, a) a) in begin
      evalVar (wkVar (keep[ a ] w) (zero {Γ}))            ≈˘⟨ id'-unit-left (evalTy a) π₂'[ evalCtx Δ ] ⟩
      id'[ evalTy a ] ∘ π₂'[ evalCtx Δ ]                  ≈˘⟨ ×'-beta-right (evalWk w ∘ π₁'[ evalTy a ]) ⟩
      evalVar (zero {Γ} {a}) ∘ evalWk (keep[ a ] w)       ∎
    evalVar-pres-∘ (keep {Δ = Δ} {b} w) (succ {Γ} {a} {b} n) = let open EqReasoning (Tm'-setoid (Δ `, b) a) in begin
      evalVar (wkVar (keep[ b ] w) (succ {Γ} {a} {b} n))  ≈⟨ ∘-pres-≈̇-left (evalVar-pres-∘ w n) π₁'[ evalTy b ] ⟩
      (evalVar n ∘ evalWk w) ∘ π₁'[ evalTy b ]            ≈⟨ ∘-assoc (evalVar n) (evalWk w) π₁'[ evalTy b ] ⟩
      evalVar n ∘ evalWk w ∘ π₁'[ evalTy b ]              ≈˘⟨ ∘-pres-≈̇-right (evalVar n) (×'-beta-left (id' ∘ π₂')) ⟩
      evalVar n ∘ π₁'[ evalTy b ] ∘ evalWk (keep[ b ] w)  ≈˘⟨ ∘-assoc (evalVar n) π₁'[ evalTy b ] (evalWk (keep[ b ] w)) ⟩
      evalVar (succ {Γ} {a} {b} n) ∘ evalWk (keep[ b ] w) ∎

abstract
  evalTm-pres-∘' : ∀ (w : Γ ⊆ Δ) (t : Tm Γ a) → evalTm (wkTm w t) ≈̇ evalTm t [ evalWk w ]'
  evalTm-pres-∘' w (var v) = evalVar-pres-∘ w v
  evalTm-pres-∘' {Δ = Δ} {a} w (lam {a = a'} t) = let open EqReasoning (Tm'-setoid Δ a) in begin
    evalTm (wkTm w (lam t))
      ≈⟨ lam'-pres-≈̇ (evalTm-pres-∘' (keep[ a' ] w) t) ⟩
    lam' (evalTm t ∘ evalWk (keep[ a' ] w))
      ≈˘⟨ lam'-nat (evalTm t) (evalWk w) ⟩
    evalTm (lam t) [ evalWk w ]'
      ∎
  evalTm-pres-∘' {Δ = Δ} {a} w (app t u) = let open EqReasoning (Tm'-setoid Δ a) in begin
    evalTm (wkTm w (app t u))
      ≈⟨ app'-pres-≈̇ (evalTm-pres-∘' w t) (evalTm-pres-∘' w u) ⟩
    app' (evalTm t ∘ evalWk w) (evalTm u ∘ evalWk w)
      ≈˘⟨ app'-nat (evalTm t) (evalTm u) (evalWk w) ⟩
    evalTm (app t u) [ evalWk w ]'
      ∎
  evalTm-pres-∘' {Δ = Δ} {a} w (letin {a = a'} t u) = let open EqReasoning (Tm'-setoid Δ a) in begin
    evalTm (wkTm w (letin t u))
      ≈⟨ letin'-pres-≈̇ (evalTm-pres-∘' w t) (evalTm-pres-∘' (keep w) u) ⟩
    letin' (evalTm t ∘ evalWk w) (evalTm u ∘ evalWk (keep[ a' ] w))
      ≈˘⟨ letin'-nat (evalTm t) (evalTm u) (evalWk w) ⟩
    evalTm (letin t u) [ evalWk w ]'
      ∎

abstract
  evalSub-pres-∘' : ∀ (σ : Sub Δ Γ) (w : Δ ⊆ Δ') → evalSub (wkSub w σ) ≈̇ evalSub σ ∘ evalWk w
  evalSub-pres-∘' []         w = ≈̇-sym []'-eta
  evalSub-pres-∘' {Γ = Γ} {Δ'} (σ `, t)   w = let open EqReasoning (Sub'-setoid Δ' Γ) in begin
    evalSub (wkSub w (σ `, t))
      ≈⟨ ⟨,⟩'-pres-≈̇ (evalSub-pres-∘' σ w) (evalTm-pres-∘' w t) ⟩
    ⟨ evalSub σ ∘ evalWk w , evalTm t ∘ evalWk w ⟩'
      ≈˘⟨ ⟨,⟩'-nat (evalSub σ) (evalTm t) (evalWk w) ⟩
    evalSub (σ `, t) ∘ evalWk w
      ∎
abstract
  evalSub-pres-∘-π₁ : ∀ (σ : Sub Δ Γ) (a : Ty) → evalSub (dropₛ {Δ} {Γ} {a} σ) ≈̇ evalSub σ ∘ π₁'[ evalTy a ]
  evalSub-pres-∘-π₁ {Δ} {Γ} σ a = let open EqReasoning (Sub'-setoid (Δ `, a) Γ) in begin
    evalSub (dropₛ {Δ} {Γ} {a} σ)       ≈⟨ evalSub-pres-∘' σ (freshWk {Δ} {a}) ⟩
    evalSub σ ∘ evalWk (freshWk {Δ} {a})  ≈⟨ ∘-pres-≈̇-right (evalSub σ) (evalWk-pres-π₁ Δ a) ⟩
    evalSub σ ∘ π₁'[ evalTy a ]         ∎

abstract
  evalSub-pres-×-map-id : ∀ (σ : Sub Δ Γ) (a : Ty) → evalSub (keepₛ {Δ} {Γ} {a} σ) ≈̇ evalSub σ ×'-map id'[ evalTy a ]
  evalSub-pres-×-map-id {Δ} {Γ} σ a = let open EqReasoning (Sub'-setoid (Δ `, a) (Γ `, a)) in begin
    evalSub (keepₛ {Δ} {Γ} {a} σ)    ≈⟨ ⟨,⟩'-pres-≈̇ (evalSub-pres-∘-π₁ σ a) (≈̇-sym (id'-unit-left (evalTy a) π₂'[ evalCtx Δ ])) ⟩
    evalSub σ ×'-map id'[ evalTy a ]  ∎

abstract
  evalSub-pres-wk : ∀ (w : Γ ⊆ Γ') → evalSub (embWk w) ≈̇ evalWk w
  evalSub-pres-wk base = []'-eta
  evalSub-pres-wk {Γ} (drop {Δ = Γ'} {a} w) = let open EqReasoning (Sub'-setoid (Γ' `, a) Γ) in begin
    evalSub (embWk (drop[ a ] w))                ≈⟨ evalSub-pres-∘' (embWk w) (freshWk {Γ'} {a}) ⟩
    evalSub (embWk w) ∘ evalWk (freshWk {Γ'} {a})  ≈⟨ ∘-pres-≈̇ (evalSub-pres-wk w) (evalWk-pres-π₁ Γ' a) ⟩
    evalWk (drop[ a ] w)                         ∎
  evalSub-pres-wk {Γ} (keep {Δ = Γ'} {a} w) = let open EqReasoning (Sub'-setoid (Γ' `, a) Γ) in begin
    evalSub (embWk (keep[ a ] w))                ≈⟨ evalSub-pres-×-map-id (embWk w) a ⟩
    evalSub (embWk w) ×'-map id'[ evalTy a ]     ≈⟨ ×'-map-pres-≈̇-left (evalSub-pres-wk w) id' ⟩
    evalWk (keep[ a ] w)                         ∎

abstract
  evalSub-pres-id : ∀ (Γ : Ctx) → evalSub idₛ[ Γ ] ≈̇ id'
  evalSub-pres-id Γ = let open EqReasoning (Sub'-setoid Γ Γ) in begin
    evalSub idₛ[ Γ ]  ≈⟨ evalSub-pres-wk idWk[ Γ ] ⟩
    evalWk idWk[ Γ ]  ≈⟨ evalWk-pres-id Γ ⟩
    id'                ∎

module _ {a : Ty} {Δ : Ctx} where
  abstract
    evalTm-pres-∘'' : ∀ (v : Var Γ a) (σ : Sub Δ Γ) → evalTm (substVar σ v) ≈̇ evalVar v [ evalSub σ ]'
    evalTm-pres-∘'' zero             (σ `, t) = ≈̇-sym (×'-beta-right (evalSub σ))
    evalTm-pres-∘'' (succ {b = b} v) (σ `, t) = let open EqReasoning (Tm'-setoid Δ a) in begin
      evalTm (substVar (σ `, t) (succ {b = b} v))     ≈⟨ evalTm-pres-∘'' v σ ⟩
      evalVar v [ evalSub σ ]'                        ≈˘⟨ ∘-pres-≈̇-right (evalVar v) (×'-beta-left (evalTm t)) ⟩
      evalVar v ∘ π₁'[ evalTy b ] ∘ evalSub (σ `, t)  ≈˘⟨ ∘-assoc (evalVar v) π₁'[ evalTy b ] (evalSub (σ `, t)) ⟩
      evalVar (succ {b = b} v) [ evalSub (σ `, t) ]'  ∎


abstract
  evalTm-pres-∘ : ∀ (t : Tm Γ a) → (σ : Sub Δ Γ) → evalTm (substTm σ t) ≈̇ evalTm t [ evalSub σ ]'
  evalTm-pres-∘ (var v) σ = evalTm-pres-∘'' v σ
  evalTm-pres-∘ {a = a} {Δ} (lam {a = a'} t) σ = let open EqReasoning (Tm'-setoid Δ a) in begin
    evalTm (substTm σ (lam t))
      ≈⟨ lam'-pres-≈̇ (evalTm-pres-∘ t (wkSub (freshWk {Δ} {a'}) σ `, var zero)) ⟩
    lam' (evalTm t [ evalSub (wkSub (freshWk {Δ} {a'}) σ `, var zero) ]')
      ≈⟨ lam'-pres-≈̇ (∘-pres-≈̇-right (evalTm t) (⟨,⟩'-pres-≈̇-left (evalSub-pres-∘' σ (freshWk {Δ} {a'})) π₂'[ evalCtx Δ ])) ⟩
    lam' (evalTm t [ ⟨ evalSub σ ∘ evalWk (freshWk {Δ} {a'}) , π₂'[ evalCtx Δ ] ⟩' ]' )
      ≈⟨ lam'-pres-≈̇ (∘-pres-≈̇-right (evalTm t) (⟨,⟩'-pres-≈̇-left (∘-pres-≈̇-right (evalSub σ) (evalWk-pres-π₁ Δ a')) π₂'[ evalCtx Δ ])) ⟩
    lam' (evalTm t [ ⟨ evalSub σ ∘ π₁'[ evalTy a' ] , π₂'[ evalCtx Δ ] ⟩' ]')
      ≈˘⟨ lam'-pres-≈̇ (∘-pres-≈̇-right (evalTm t) (⟨,⟩'-pres-≈̇-right (evalSub σ ∘ π₁'[ evalTy a' ]) (id'-unit-left (evalTy a') π₂'[ evalCtx Δ ]))) ⟩
    lam' (evalTm t ∘ evalSub σ ×'-map id'[ evalTy a' ])
      ≈˘⟨ lam'-nat (evalTm t) (evalSub σ) ⟩
    evalTm (lam t) [ evalSub σ ]'
      ∎
  evalTm-pres-∘ {a = a} {Δ} (app t u) σ = let open EqReasoning (Tm'-setoid Δ a) in begin
    evalTm (substTm σ (app t u))
      ≈⟨ app'-pres-≈̇ (evalTm-pres-∘ t σ) (evalTm-pres-∘ u σ) ⟩
    app' (evalTm t [ evalSub σ ]') (evalTm u [ evalSub σ ]')
      ≈˘⟨ app'-nat (evalTm t) (evalTm u) (evalSub σ) ⟩
    evalTm (app t u) [ evalSub σ ]'
      ∎
  evalTm-pres-∘ {a = a} {Δ} (letin {a = a'} t u) σ = let open EqReasoning (Tm'-setoid Δ a) in begin
    evalTm (substTm σ (letin t u))
      ≈⟨ letin'-pres-≈̇ (evalTm-pres-∘ t σ) (evalTm-pres-∘ u (keepₛ σ)) ⟩
    letin' (evalTm t [ evalSub σ ]') (evalTm u [ evalSub (wkSub (freshWk {Δ} {a'}) σ `, var zero) ]')
      ≈⟨ letin'-pres-≈̇-right _ (∘-pres-≈̇-right (evalTm u) (⟨,⟩'-pres-≈̇-left (evalSub-pres-∘' σ (freshWk {Δ} {a'})) π₂'[ evalCtx Δ ])) ⟩
    letin' (evalTm t [ evalSub σ ]') (evalTm u [ ⟨ evalSub σ ∘ evalWk (freshWk {Δ} {a'}) , π₂'[ evalCtx Δ ] ⟩' ]')
      ≈⟨ letin'-pres-≈̇-right _ ((∘-pres-≈̇-right (evalTm u) (⟨,⟩'-pres-≈̇-left (∘-pres-≈̇-right (evalSub σ) (evalWk-pres-π₁ Δ a')) π₂'[ evalCtx Δ ]))) ⟩
    letin' (evalTm t [ evalSub σ ]') (evalTm u [ ⟨ evalSub σ ∘ π₁'[ evalTy a' ] , π₂'[ evalCtx Δ ] ⟩' ]')
      ≈˘⟨ letin'-pres-≈̇-right _ (∘-pres-≈̇-right (evalTm u) ((⟨,⟩'-pres-≈̇-right (evalSub σ ∘ π₁'[ evalTy a' ]) (id'-unit-left (evalTy a') π₂'[ evalCtx Δ ])))) ⟩
    letin' (evalTm t [ evalSub σ ]') (evalTm u [ (evalSub σ) ×'-map id'[ evalTy a' ]  ]')
      ≈˘⟨ letin'-nat (evalTm t) (evalTm u) (evalSub σ) ⟩
    (evalTm (letin t u) [ evalSub σ ]')
      ∎

abstract
  evalTm-sound : (s : t ⟶ t') → evalTm t ≈̇ evalTm t'
  evalTm-sound (red-fun {Γ} {a} {b} t u) = let open EqReasoning (Tm'-setoid Γ b) in begin
    evalTm (app (lam t) u)
      ≈⟨ ⇒'-beta (evalTm t) (evalTm u) ⟩
    evalTm t [ ⟨ id'[ evalCtx Γ ] , evalTm u ⟩' ]'
      ≈˘⟨ ∘-pres-≈̇-right (evalTm t) (⟨,⟩'-pres-≈̇-left (evalSub-pres-id Γ) (evalTm u)) ⟩
    evalTm t [ ⟨ evalSub idₛ[ Γ ] , evalTm u ⟩' ]'
      ≈˘⟨ evalTm-pres-∘ t (idₛ `, u) ⟩
    evalTm (substTm (idₛ[ Γ ] `, u) t)
      ∎
  evalTm-sound (exp-fun {Γ} {a} {b} t) = let open EqReasoning (Tm'-setoid Γ (a ⇒ b)) in begin
    evalTm t
      ≈⟨ ⇒'-eta (evalTm t) ⟩
    lam' (app' (evalTm t [ π₁'[ evalTy a ] ]') π₂'[ evalCtx Γ ])
      ≈˘⟨ lam'-pres-≈̇ (app'-pres-≈̇-left (∘-pres-≈̇-right (evalTm t) (evalWk-pres-π₁ Γ a)) π₂'[ evalCtx Γ ]) ⟩
    lam' (app' (evalTm t [ evalWk (freshWk {Γ} {a}) ]') π₂'[ evalCtx Γ ])
      ≈˘⟨ lam'-pres-≈̇ (app'-pres-≈̇-left (evalTm-pres-∘' freshWk t) π₂'[ evalCtx Γ ]) ⟩
    evalTm (lam (app (wkTm freshWk t) (var zero)))
      ∎
  evalTm-sound (red-circ {Γ} {a} {b} {c} t u u') = let open EqReasoning (Tm'-setoid Γ (◯ c)) in begin
    evalTm (letin (letin t u) u')
      ≈⟨ ◯'-beta (evalTm t) (evalTm u) (evalTm u') ⟩
    letin' (evalTm t) (evalTm u' [ ⟨ π₁'[ evalTy a ] , evalTm u ⟩' ]')
      ≈˘⟨ letin'-pres-≈̇-right (evalTm t) (∘-pres-≈̇-right (evalTm u') (⟨,⟩'-pres-≈̇-left (id'-unit-left (evalCtx Γ) π₁'[ evalTy a ]) (evalTm u))) ⟩
    letin' (evalTm t) (evalTm u' [ ⟨ id' ∘ π₁'[ evalTy a ] , evalTm u ⟩' ]' )
      ≈˘⟨ letin'-pres-≈̇-right (evalTm t) (∘-pres-≈̇-right (evalTm u') (⟨,⟩'-pres-≈̇-left (∘-pres-≈̇ (evalSub-pres-id Γ) (≈̇-trans (∘-pres-≈̇-left (evalWk-pres-id Γ) π₁') (id'-unit-left (evalCtx Γ) π₁'))) (evalTm u))) ⟩
    letin' (evalTm t) (evalTm u' [ ⟨ evalSub idₛ[ Γ ] ∘ evalWk (freshWk {Γ = Γ} {a = a}) , evalTm u ⟩' ]' )
      ≈˘⟨ letin'-pres-≈̇-right (evalTm t) (∘-pres-≈̇-right (evalTm u') (⟨,⟩'-pres-≈̇-left (evalSub-pres-∘' idₛ[ Γ ] freshWk) (evalTm u))) ⟩
    letin' (evalTm t) (evalTm u' [ evalSub (wkSub freshWk (idₛ[ Γ ]) `, u) ]' )
      ≈˘⟨ letin'-pres-≈̇-right (evalTm t) (evalTm-pres-∘ u' (wkSub freshWk idₛ `, u)) ⟩
    letin' (evalTm t) (evalTm (substTm (wkSub freshWk (idₛ[ Γ ]) `, u) u'))
       ≡⟨⟩
    (evalTm (letin t (substTm (wkSub freshWk idₛ `, u) u'))) ∎
  evalTm-sound (exp-circ {Γ} {a} t) = let open EqReasoning (Tm'-setoid Γ (◯ a)) in begin
    evalTm t
      ≈⟨ ◯'-eta (evalTm t) ⟩
    letin' (evalTm t) π₂'[ evalCtx Γ ]
      ≡⟨⟩
    evalTm (letin t (var zero))
      ∎
  evalTm-sound (cong-lam s)            = lam'-pres-≈̇        (evalTm-sound s)
  evalTm-sound (cong-app1 {u = u} s)   = app'-pres-≈̇-left   (evalTm-sound s) (evalTm u)
  evalTm-sound (cong-app2 {t = t} s)   = app'-pres-≈̇-right  (evalTm t) (evalTm-sound s)
  evalTm-sound (cong-letin1 {u = u} s) = letin'-pres-≈̇-left   (evalTm-sound s) (evalTm u)
  evalTm-sound (cong-letin2 {t = t} s) = letin'-pres-≈̇-right  (evalTm t) (evalTm-sound s)
